experiment/Experiment.Steel.Repr.SF_to_Fun.fst
@@ -40,6 +40,14 @@ let sl_tys_lam_id ()
   assert (Fun.tys_lam_id #s lm)
     by T.(norm [delta_only [`%Fun.tys_lam_id; `%sl_tys; `%Fun.Mktys'?.t; `%Fun.Mktys'?.v]])
 
+unfold
+let add_sl_to_wp (#a : Type u#a) (wp : pure_wp a) : pure_wp ((sl_tys u#a u#b).v ({val_t = a; sel_t = (fun _ -> [])}))
+  =
+    (**) FStar.Monotonic.Pure.elim_pure_wp_monotonicity wp;
+    FStar.Monotonic.Pure.as_pure_wp (fun pt ->
+      wp (fun (x : a) -> pt ({val_v = x; sel_v = Fl.nil})))
+
+
 //FIXME this proof succeeds in interactive mode with --fuel 1 but not in batch mode
 //      (both wihout hints)
 #push-options "--z3rlimit 40 --ifuel 1 --fuel 2"
@@ -103,20 +111,11 @@ and repr_Fun_of_SF_ens #val_t #sel_t (t : prog_tree val_t sel_t)
               == (exists (x : a) . as_ensures wp x /\ tree_ens (g x) val_v sel_v))
             by T.(trefl ());
           assert (Fun.tree_ens (repr_Fun_of_SF (TbindP a b post wp g)) ({val_v; sel_v})
-              <==> (exists (x : a) .
-                   (exists (nl : Fl.flist []) . as_ensures (add_sl_to_wp wp) ({val_v = x; sel_v = nl})) /\
-                   Fun.tree_ens (repr_Fun_of_SF (g x)) ({val_v; sel_v})))
-            by T.(norm [delta_only [`%Fun.tree_ens; `%repr_Fun_of_SF; `%sl_uncurrify;
-                                    `%sl_tys; `%sl_tys'; `%Fun.Mktys'?.ex; `%sl_ex;
-                                    `%Mksl_tys_t?.val_t; `%Mksl_tys_t?.sel_t];
-                        iota; zeta]; smt ());
+              == (exists (x : a) . as_ensures wp x /\ Fun.tree_ens (repr_Fun_of_SF (g x)) ({val_v; sel_v})))
+            by T.(trefl ());
           introduce forall (x : a) .
-              ((exists (nl : Fl.flist []) . as_ensures (add_sl_to_wp wp) ({val_v = x; sel_v = nl})) <==>
-                  as_ensures wp x) /\
-              (tree_ens (g x) val_v sel_v <==> Fun.tree_ens (repr_Fun_of_SF (g x)) ({val_v; sel_v}))
-            with introduce _ /\ _
-            with FStar.Monotonic.Pure.elim_pure_wp_monotonicity wp
-             and repr_Fun_of_SF_ens (g x) val_v sel_v
+                    (tree_ens (g x) val_v sel_v <==> Fun.tree_ens (repr_Fun_of_SF (g x)) ({val_v; sel_v}))
+            with repr_Fun_of_SF_ens (g x) val_v sel_v
   | Tif a guard post thn els ->
           if guard
           then repr_Fun_of_SF_ens thn val_v sel_v
